commented the transitivity and narrowing proof

src/HOL/Nominal/Examples/Fsub.thy
@@ -14,11 +14,11 @@ text{* Authors: Christian Urban,
 
        with great help from Stefan Berghofer and  Markus Wenzel. *}
 
-section {* Atom Types, Types and Terms *}
+section {* Types for Names, Nominal Datatype Declaration for Types and Terms *}
 
 text {* The main point of this solution is to use names everywhere (be they bound, 
-  binding or free). There are two kinds of names corresponding to type-variables and 
-  to term-variables in System \FSUB. These two kinds of names are represented in 
+  binding or free). In System \FSUB{} there are two kinds of names corresponding to 
+  type-variables and to term-variables. These two kinds of names are represented in 
   the nominal datatype package as atom-types @{text "tyvrs"} and @{text "vrs"}: *}
 
 atom_decl tyvrs vrs
@@ -44,9 +44,9 @@ nominal_datatype trm =
   | Tapp  "trm" "ty"
 
 text {* To be polite to the eye, some more familiar notation is introduced. 
-  Because of the change in the order of the argument, one needs to use 
+  Because of the change in the order of arguments, one needs to use 
   translation rules, instead of syntax annotations at the term-constructors
-  like for @{term "Arrow"}. *}
+  as given for @{term "Arrow"}. *}
 
 syntax
   Forall_syn :: "tyvrs \<Rightarrow> ty \<Rightarrow> ty \<Rightarrow> ty" ("\<forall>[_<:_]._" [100,100,100] 100)
@@ -58,9 +58,11 @@ translations
   "Lam [x:T].t" \<rightleftharpoons> "trm.Lam x t T"
   "Tabs [X<:T].t" \<rightleftharpoons> "trm.Tabs X t T"
 
-text {* Note that the nominal-datatype declarations for @{typ "ty"} and @{typ "trm"}
-  do \emph{not} define "classical" constructor-based datatypes, but rather define
-  $\alpha$-equivalence classes. Indeed we can show that $\alpha$-equivalent @{typ "ty"}s 
+text {* Again there are numerous facts that are proved automatically for @{typ "ty"} 
+  and @{typ "trm"}: for example that the set of free variables, i.e.~@{text "support"}, 
+  is only finite. However note that nominal-datatype declarations do \emph{not} define 
+  "classical" constructor-based datatypes, but rather define $\alpha$-equivalence 
+  classes---we can for example show that $\alpha$-equivalent @{typ "ty"}s 
   and @{typ "trm"}s are equal: *}
 
 lemma alpha_illustration:
@@ -68,15 +70,16 @@ lemma alpha_illustration:
   and "Lam [x:T].(Var x) = Lam [y:T].(Var y)"
   by (simp_all add: ty.inject trm.inject alpha calc_atm fresh_atm)
 
-section {* Typing Contexts *}
+section {* SubTyping Contexts *}
 
 types ty_context = "(tyvrs\<times>ty) list"
 
-text {* Typing contexts are represented as lists "growing" on the left, 
-  in contrast to the POPLmark-paper. *}
+text {* Typing contexts are represented as lists "growing" on the left; we
+  thereby deviating from the convention in the POPLmark-paper. The lists contain
+  pairs of type-variables and types. *}
 
-text {* In order to state valitity-conditions for typing-context, the notion of
-  a domain of a typing-context is handy. *}
+text {* In order to state valitity-conditions for typing-contexts, the notion of
+  a @{text "domain"} of a typing-context is handy. *}
 
 consts
   "domain" :: "ty_context \<Rightarrow> tyvrs set"
@@ -93,6 +96,10 @@ lemma finite_domain:
   shows "finite (domain \<Gamma>)"
   by (induct \<Gamma>, auto)
 
+lemma domain_supp:
+  shows "(supp (domain \<Gamma>)) = (domain \<Gamma>)"
+  by (simp only: at_fin_set_supp at_tyvrs_inst finite_domain)
+
 lemma domain_inclusion:
   assumes a: "(X,T)\<in>set \<Gamma>" 
   shows "X\<in>(domain \<Gamma>)"
@@ -107,18 +114,31 @@ lemma domain_append:
   shows "domain (\<Gamma>@\<Delta>) = ((domain \<Gamma>) \<union> (domain \<Delta>))"
   by (induct \<Gamma>, auto)
 
+lemma fresh_domain_cons:
+  fixes X::"tyvrs"
+  shows "X\<sharp>(domain (Y#\<Gamma>)) = (X\<sharp>(fst Y) \<and> X\<sharp>(domain \<Gamma>))"
+  by (simp add: fresh_fin_insert pt_tyvrs_inst at_tyvrs_inst fs_tyvrs_inst finite_domain)
+
+lemma fresh_domain:
+  fixes X::"tyvrs"
+  assumes a: "X\<sharp>\<Gamma>" 
+  shows "X\<sharp>(domain \<Gamma>)"
+using a
+apply(induct \<Gamma>)
+apply(simp add: fresh_set_empty) 
+apply(simp only: fresh_domain_cons)
+apply(auto simp add: fresh_prod fresh_list_cons) 
+done
+
 text {* Not all lists of type @{typ "ty_context"} are well-formed. One condition
   requires that in @{term "(X,S)#\<Gamma>"} all free variables of @{term "S"} must be 
-  in @{term "domain \<Gamma>"},  that is @{term "S"} must be closed in @{term "\<Gamma>"}. *}
+  in the @{term "domain"} of @{term "\<Gamma>"}, that is @{term "S"} must be @{text "closed"} 
+  in @{term "\<Gamma>"}. The set of free variables of @{term "S"} is defined as the 
+  @{text "support"} of @{term "S"}. *}
 
 constdefs
   "closed_in" :: "ty \<Rightarrow> ty_context \<Rightarrow> bool" ("_ closed'_in _" [100,100] 100)
   "S closed_in \<Gamma> \<equiv> (supp S)\<subseteq>(domain \<Gamma>)"
-
-lemma closed_in_def2:
-  shows "(S closed_in \<Gamma>) = ((supp S)\<subseteq>((supp (domain \<Gamma>))::tyvrs set))"
-apply(simp add: closed_in_def at_fin_set_supp[OF at_tyvrs_inst, OF finite_domain])
-done
 
 lemma closed_in_eqvt:
   fixes pi::"tyvrs prm"
@@ -133,6 +153,8 @@ proof (unfold "closed_in_def")
     by (simp add: domain_eqvt pt_perm_supp[OF pt_tyvrs_inst, OF at_tyvrs_inst])
 qed
 
+text {* Now validity of a context is a straightforward inductive definition. *}
+  
 consts
   valid_rel :: "ty_context set" 
   valid_sym :: "ty_context \<Rightarrow> bool" ("\<turnstile> _ ok" [100] 100)
@@ -140,9 +162,8 @@ translations
   "\<turnstile> \<Gamma> ok" \<rightleftharpoons> "\<Gamma> \<in> valid_rel"  
 inductive valid_rel
 intros
-v_nil[intro]:  "\<turnstile> [] ok"
-v_cons[intro]: "\<lbrakk>\<turnstile> \<Gamma> ok; X\<sharp>\<Gamma>; T closed_in \<Gamma>\<rbrakk>  \<Longrightarrow>  \<turnstile> ((X,T)#\<Gamma>) ok"
-
+valid_nil[simp]:  "\<turnstile> [] ok"
+valid_cons[simp]: "\<lbrakk>\<turnstile> \<Gamma> ok; X\<sharp>(domain \<Gamma>); T closed_in \<Gamma>\<rbrakk>  \<Longrightarrow>  \<turnstile> ((X,T)#\<Gamma>) ok"
 
 lemma valid_eqvt:
   fixes pi::"tyvrs prm"
@@ -150,23 +171,23 @@ lemma valid_eqvt:
   shows "\<turnstile> (pi\<bullet>\<Gamma>) ok"
   using a
 proof (induct)
-  case v_nil
-  show "\<turnstile> (pi\<bullet>[]) ok" by (simp add: valid_rel.v_nil)
+  case valid_nil
+  show "\<turnstile> (pi\<bullet>[]) ok" by simp
 next
-  case (v_cons T X \<Gamma>)
-  have "\<turnstile> (pi \<bullet> \<Gamma>) ok" by fact
+  case (valid_cons T X \<Gamma>)
+  have "\<turnstile> (pi\<bullet>\<Gamma>) ok" by fact
   moreover
-  have "X\<sharp>\<Gamma>" by fact
-  hence "(pi\<bullet>X)\<sharp>(pi\<bullet>\<Gamma>)" by (simp add: fresh_eqvt)
+  have "X\<sharp>(domain \<Gamma>)" by fact
+  hence "(pi\<bullet>X)\<sharp>(domain (pi\<bullet>\<Gamma>))" by (simp add: fresh_eqvt domain_eqvt[symmetric])
   moreover
   have "T closed_in \<Gamma>" by fact
-  hence "(pi\<bullet>T) closed_in (pi\<bullet>\<Gamma>)" by (rule closed_in_eqvt)
-  ultimately show "\<turnstile> (pi\<bullet>((X,T)#\<Gamma>)) ok" by (simp add: valid_rel.v_cons)
+  hence "(pi\<bullet>T) closed_in (pi\<bullet>\<Gamma>)" by (simp add: closed_in_eqvt)
+  ultimately show "\<turnstile> (pi\<bullet>((X,T)#\<Gamma>)) ok" by simp
 qed
 
 lemma validE:
   assumes a: "\<turnstile> ((X,T)#\<Gamma>) ok"
-  shows "\<turnstile> \<Gamma> ok \<and> X\<sharp>\<Gamma> \<and> T closed_in \<Gamma>"
+  shows "\<turnstile> \<Gamma> ok \<and> X\<sharp>(domain \<Gamma>) \<and> T closed_in \<Gamma>"
 using a by (cases, auto)
 
 lemma validE_append:
@@ -174,74 +195,61 @@ lemma validE_append:
   shows "\<turnstile> \<Gamma> ok"
   using a by (induct \<Delta>, auto dest: validE)
 
-lemma domain_fresh:
-  fixes X::"tyvrs"
-  assumes a: "\<turnstile> \<Gamma> ok" 
-  shows "X\<sharp>(domain \<Gamma>) = X\<sharp>\<Gamma>"
-using a
-apply(induct \<Gamma>)
-apply(auto simp add: fresh_list_nil fresh_list_cons fresh_set_empty fresh_prod fresh_atm
-  fresh_fin_insert[OF pt_tyvrs_inst, OF at_tyvrs_inst, OF fs_tyvrs_inst, OF finite_domain])
-apply(force simp add: closed_in_def2 fresh_def)
-done
-
 lemma closed_in_fresh:
   fixes X::"tyvrs"
-  assumes a1: "S closed_in \<Gamma>"
-  and     a2: "X\<sharp>\<Gamma>" 
-  and     a3: "\<turnstile> \<Gamma> ok"
+  assumes a: "S closed_in \<Gamma>"
+  and     b: "X\<sharp>(domain \<Gamma>)" 
+  and     c: "\<turnstile> \<Gamma> ok"
   shows "X\<sharp>S"
-using a1 a2 a3
-apply(simp add: closed_in_def2)
-apply(simp add: domain_fresh[symmetric])
-apply(simp add: fresh_def)
-apply(force)
-done
+using a b c by (force simp add: fresh_def domain_supp closed_in_def)
 
 lemma replace_type:
   assumes a: "\<turnstile> (\<Delta>@(X,T)#\<Gamma>) ok"
   and     b: "S closed_in \<Gamma>"
   shows "\<turnstile> (\<Delta>@(X,S)#\<Gamma>) ok"
-using a b 
+using a b
 apply(induct \<Delta>)
-apply(auto dest!: validE intro!: v_cons simp add: fresh_list_append fresh_list_cons fresh_prod)
-apply(drule validE_append)
-apply(drule validE)
-apply(drule_tac S="S" in closed_in_fresh)
-apply(simp)
-apply(force)+
-apply(simp add: closed_in_def2)
-apply(simp add: domain_append)
+apply(auto dest!: validE intro!: valid_cons simp add: domain_append closed_in_def)
 done
 
-lemma fresh_implies_not_member:
-  fixes \<Gamma>::"ty_context"
-  assumes a: "X\<sharp>\<Gamma>" 
-  shows "\<not>(\<exists>T.(X,T)\<in>(set \<Gamma>))"
-  using a by (induct \<Gamma>, auto dest: validE simp add: fresh_list_cons fresh_prod fresh_atm)
- 
 lemma uniqueness_of_ctxt:
   fixes \<Gamma>::"ty_context"
   assumes a: "\<turnstile> \<Gamma> ok"
   and     b: "(X,T)\<in>set \<Gamma>"
   and     c: "(X,S)\<in>set \<Gamma>"
   shows "T=S"
-  using a b c by (induct \<Gamma>, auto dest: validE fresh_implies_not_member)
+using a b c
+proof (induct)
+  case valid_nil thus "T=S" by simp
+next
+  case (valid_cons U Y \<Gamma>)
+  moreover
+  { fix \<Gamma>::"ty_context"
+    assume a: "X\<sharp>(domain \<Gamma>)" 
+    have "\<not>(\<exists>T.(X,T)\<in>(set \<Gamma>))" using a 
+    proof (induct \<Gamma>)
+      case (Cons Y \<Gamma>)
+      thus "\<not> (\<exists>T.(X,T)\<in>set(Y#\<Gamma>))" 
+	by (simp only: fresh_domain_cons, auto simp add: fresh_atm)
+    qed (simp)
+  }
+  ultimately show "T=S" by auto
+qed 
 
-subsection {* Size Functions and Capture-Avoiding Substitutiuon for Types *}
+section {* Size and Capture-Avoiding Substitutiuon for Types *}
 
-text {* In the current version of the nominal datatype 
-  package even simple functions (such as size of types and capture-avoiding
-  substitution) can only be defined manually via some sophisticated proof 
-  constructions. Therefore we sill just assume them here. *}
+text {* In the current version of the nominal datatype-package even simple 
+  functions (such as size of types and capture-avoiding substitution) can 
+  only be defined manually via some labourious proof constructions. Therefore 
+  we sill just assume them here. *}
 
 consts size_ty :: "ty \<Rightarrow> nat"
 
 lemma size_ty[simp]:
   shows "size_ty (Tvar X) = 1"
   and   "size_ty (Top) = 1"
-  and   "\<lbrakk>size_ty t\<^isub>1 = m ; size_ty t\<^isub>2 = n\<rbrakk> \<Longrightarrow> size_ty (t\<^isub>1 \<rightarrow> t\<^isub>2) = m + n + 1"
-  and   "\<lbrakk>size_ty t\<^isub>1 = m ; size_ty t\<^isub>2 = n\<rbrakk> \<Longrightarrow> size_ty (\<forall>[a<:t\<^isub>1].t\<^isub>2) = m + n + 1"
+  and   "\<lbrakk>size_ty T\<^isub>1 = m; size_ty T\<^isub>2 = n\<rbrakk> \<Longrightarrow> size_ty (T\<^isub>1 \<rightarrow> T\<^isub>2) = m + n + 1"
+  and   "\<lbrakk>size_ty T\<^isub>1 = m; size_ty T\<^isub>2 = n\<rbrakk> \<Longrightarrow> size_ty (\<forall>[X<:T\<^isub>1].T\<^isub>2) = m + n + 1"
 sorry
 
 consts subst_ty :: "ty \<Rightarrow> tyvrs \<Rightarrow> ty \<Rightarrow> ty" ("_[_:=_]\<^isub>t\<^isub>y" [100,100,100] 100)
@@ -254,7 +262,7 @@ lemma subst_ty[simp]:
   and   "\<lbrakk>X\<sharp>Y; X\<sharp>T\<rbrakk> \<Longrightarrow> (\<forall>[X<:T\<^isub>1].T\<^isub>2)[Y:=T]\<^isub>t\<^isub>y = (\<forall>[X<:(T\<^isub>1[Y:=T]\<^isub>t\<^isub>y)].(T\<^isub>2[Y:=T]\<^isub>t\<^isub>y))"
 sorry
 
-consts subst_ctxt :: "ty_context \<Rightarrow> tyvrs \<Rightarrow> ty \<Rightarrow> ty_context" ("_[_:=_]\<^isub>t\<^isub>y\<^isub>c" [100,100,100] 100)
+consts subst_tyc :: "ty_context \<Rightarrow> tyvrs \<Rightarrow> ty \<Rightarrow> ty_context" ("_[_:=_]\<^isub>t\<^isub>y\<^isub>c" [100,100,100] 100)
 primrec
 "([])[Y:=T]\<^isub>t\<^isub>y\<^isub>c= []"
 "(XT#\<Gamma>)[Y:=T]\<^isub>t\<^isub>y\<^isub>c = (fst XT,(snd XT)[Y:=T]\<^isub>t\<^isub>y)#(\<Gamma>[Y:=T]\<^isub>t\<^isub>y\<^isub>c)"
@@ -264,18 +272,18 @@ section {* Subtyping-Relation *}
 consts
   subtype_of :: "(ty_context \<times> ty \<times> ty) set"   
 syntax 
-  subtype_of_syn :: "ty_context \<Rightarrow> ty \<Rightarrow> ty \<Rightarrow> bool"   ("_ \<turnstile> _ <: _" [100,100,100] 100)
+  subtype_of_syn :: "ty_context \<Rightarrow> ty \<Rightarrow> ty \<Rightarrow> bool"   ("_\<turnstile>_<:_" [100,100,100] 100)
 
 translations
   "\<Gamma> \<turnstile> S <: T" \<rightleftharpoons> "(\<Gamma>,S,T) \<in> subtype_of"
 inductive subtype_of
 intros
-S_Top[intro]:   "\<lbrakk>\<turnstile> \<Gamma> ok; S closed_in \<Gamma>\<rbrakk> \<Longrightarrow> \<Gamma> \<turnstile> S <: Top"
-S_Var[intro]:   "\<lbrakk>\<turnstile> \<Gamma> ok; (X,S) \<in> set \<Gamma>; \<Gamma> \<turnstile> S <: T\<rbrakk> \<Longrightarrow> \<Gamma> \<turnstile> (Tvar X) <: T"
-S_Refl[intro]:  "\<lbrakk>\<turnstile> \<Gamma> ok; X \<in> domain \<Gamma>\<rbrakk>\<Longrightarrow> \<Gamma> \<turnstile> Tvar X <: Tvar X"
-S_Arrow[intro]: "\<lbrakk>\<Gamma> \<turnstile> T\<^isub>1 <: S\<^isub>1; \<Gamma> \<turnstile> S\<^isub>2 <: T\<^isub>2\<rbrakk> \<Longrightarrow> \<Gamma> \<turnstile> (S\<^isub>1 \<rightarrow> S\<^isub>2) <: (T\<^isub>1 \<rightarrow> T\<^isub>2)" 
-S_All[intro]:   "\<lbrakk>\<Gamma> \<turnstile> T\<^isub>1 <: S\<^isub>1; X\<sharp>\<Gamma>; ((X,T\<^isub>1)#\<Gamma>) \<turnstile> S\<^isub>2 <: T\<^isub>2\<rbrakk> 
-                  \<Longrightarrow> \<Gamma> \<turnstile> \<forall>[X<:S\<^isub>1].S\<^isub>2 <: \<forall>[X<:T\<^isub>1].T\<^isub>2"  
+S_Top[intro]:    "\<lbrakk>\<turnstile> \<Gamma> ok; S closed_in \<Gamma>\<rbrakk> \<Longrightarrow> \<Gamma> \<turnstile> S <: Top"
+S_Var[intro]:    "\<lbrakk>(X,S) \<in> set \<Gamma>; \<Gamma> \<turnstile> S <: T\<rbrakk> \<Longrightarrow> \<Gamma> \<turnstile> (Tvar X) <: T"
+S_Refl[intro]:   "\<lbrakk>\<turnstile> \<Gamma> ok; X \<in> domain \<Gamma>\<rbrakk>\<Longrightarrow> \<Gamma> \<turnstile> Tvar X <: Tvar X"
+S_Arrow[intro]:  "\<lbrakk>\<Gamma> \<turnstile> T\<^isub>1 <: S\<^isub>1; \<Gamma> \<turnstile> S\<^isub>2 <: T\<^isub>2\<rbrakk> \<Longrightarrow> \<Gamma> \<turnstile> (S\<^isub>1 \<rightarrow> S\<^isub>2) <: (T\<^isub>1 \<rightarrow> T\<^isub>2)" 
+S_Forall[intro]: "\<lbrakk>\<Gamma> \<turnstile> T\<^isub>1 <: S\<^isub>1; X\<sharp>\<Gamma>; ((X,T\<^isub>1)#\<Gamma>) \<turnstile> S\<^isub>2 <: T\<^isub>2\<rbrakk> 
+                 \<Longrightarrow> \<Gamma> \<turnstile> \<forall>[X<:S\<^isub>1].S\<^isub>2 <: \<forall>[X<:T\<^isub>1].T\<^isub>2"  
 
 lemma subtype_implies_closed:
   assumes a: "\<Gamma> \<turnstile> S <: T"
@@ -311,11 +319,11 @@ lemma subtype_implies_fresh:
   shows "X\<sharp>S \<and> X\<sharp>T"  
 proof -
   from a1 have "\<turnstile> \<Gamma> ok" by (rule subtype_implies_ok)
-  with a2 have "X\<sharp>domain(\<Gamma>)" by (simp add: domain_fresh)
+  with a2 have "X\<sharp>domain(\<Gamma>)" by (simp add: fresh_domain)
   moreover
   from a1 have "S closed_in \<Gamma> \<and> T closed_in \<Gamma>" by (rule subtype_implies_closed)
   hence "supp S \<subseteq> ((supp (domain \<Gamma>))::tyvrs set)" 
-    and "supp T \<subseteq> ((supp (domain \<Gamma>))::tyvrs set)" by (simp_all add: closed_in_def2)
+    and "supp T \<subseteq> ((supp (domain \<Gamma>))::tyvrs set)" by (simp_all add: domain_supp closed_in_def)
   ultimately show "X\<sharp>S \<and> X\<sharp>T" by (force simp add: supp_prod fresh_def)
 qed
 
@@ -344,20 +352,20 @@ apply(force intro: valid_eqvt closed_in_eqvt)
 apply(force intro: closed_in_eqvt valid_eqvt silly_eqvt1)
 apply(force intro: valid_eqvt silly_eqvt2)
 apply(force)
-apply(force intro!: S_All simp add: fresh_prod fresh_eqvt)
+apply(force intro!: S_Forall simp add: fresh_prod fresh_eqvt)
 done
 
-lemma subtype_of_induct[consumes 1, case_names S_Top S_Var S_Refl S_Arrow S_All]:
+lemma subtype_of_induct[consumes 1, case_names S_Top S_Var S_Refl S_Arrow S_Forall]:
   fixes  P :: "'a::fs_tyvrs\<Rightarrow>ty_context \<Rightarrow> ty \<Rightarrow> ty \<Rightarrow>bool"
   assumes a: "\<Gamma> \<turnstile> S <: T"
-  and a1: "\<And>\<Gamma> S x. \<turnstile> \<Gamma> ok \<Longrightarrow> S closed_in \<Gamma> \<Longrightarrow> P x \<Gamma> S Top"
-  and a2: "\<And>\<Gamma> X S T x. \<turnstile> \<Gamma> ok \<Longrightarrow> (X,S)\<in>set \<Gamma> \<Longrightarrow> \<Gamma> \<turnstile> S <: T \<Longrightarrow> (\<And>z. P z \<Gamma> S T)
-    \<Longrightarrow> P x \<Gamma> (Tvar X) T"
-  and a3: "\<And>\<Gamma> X x. \<turnstile> \<Gamma> ok \<Longrightarrow> X\<in>domain \<Gamma> \<Longrightarrow> P x \<Gamma> (Tvar X) (Tvar X)"  
-  and a4: "\<And>\<Gamma> S\<^isub>1 S\<^isub>2 T\<^isub>1 T\<^isub>2 x. \<Gamma> \<turnstile> T\<^isub>1 <: S\<^isub>1 \<Longrightarrow> (\<And>z. P z \<Gamma> T\<^isub>1 S\<^isub>1) \<Longrightarrow> \<Gamma> \<turnstile> S\<^isub>2 <: T\<^isub>2 \<Longrightarrow> 
-    (\<And>z. P z \<Gamma> S\<^isub>2 T\<^isub>2) \<Longrightarrow> P x \<Gamma> (S\<^isub>1 \<rightarrow> S\<^isub>2) (T\<^isub>1 \<rightarrow> T\<^isub>2)"
-  and a5: "\<And>\<Gamma> X S\<^isub>1 S\<^isub>2 T\<^isub>1 T\<^isub>2 x. X\<sharp>x \<Longrightarrow> X\<sharp>(\<Gamma>,S\<^isub>1,T\<^isub>1) \<Longrightarrow> \<Gamma> \<turnstile> T\<^isub>1 <: S\<^isub>1 \<Longrightarrow> (\<And>z. P z \<Gamma> T\<^isub>1 S\<^isub>1) 
-    \<Longrightarrow> ((X,T\<^isub>1)#\<Gamma>) \<turnstile> S\<^isub>2 <: T\<^isub>2 \<Longrightarrow> (\<And>z. P z ((X,T\<^isub>1)#\<Gamma>) S\<^isub>2 T\<^isub>2) \<Longrightarrow> P x \<Gamma> (\<forall>[X<:S\<^isub>1].S\<^isub>2) (\<forall>[X<:T\<^isub>1].T\<^isub>2)"
+  and a1: "\<And>\<Gamma> S x. \<lbrakk>\<turnstile> \<Gamma> ok; S closed_in \<Gamma>\<rbrakk> \<Longrightarrow> P x \<Gamma> S Top"
+  and a2: "\<And>\<Gamma> X S T x. \<lbrakk>(X,S)\<in>set \<Gamma>; \<Gamma> \<turnstile> S <: T; \<And>z. P z \<Gamma> S T\<rbrakk> \<Longrightarrow> P x \<Gamma> (Tvar X) T"
+  and a3: "\<And>\<Gamma> X x. \<lbrakk>\<turnstile> \<Gamma> ok; X\<in>domain \<Gamma>\<rbrakk> \<Longrightarrow> P x \<Gamma> (Tvar X) (Tvar X)"  
+  and a4: "\<And>\<Gamma> S\<^isub>1 S\<^isub>2 T\<^isub>1 T\<^isub>2 x. \<lbrakk>\<Gamma> \<turnstile> T\<^isub>1 <: S\<^isub>1; \<And>z. P z \<Gamma> T\<^isub>1 S\<^isub>1; \<Gamma> \<turnstile> S\<^isub>2 <: T\<^isub>2; \<And>z. P z \<Gamma> S\<^isub>2 T\<^isub>2\<rbrakk> 
+  \<Longrightarrow> P x \<Gamma> (S\<^isub>1 \<rightarrow> S\<^isub>2) (T\<^isub>1 \<rightarrow> T\<^isub>2)"
+  and a5: "\<And>\<Gamma> X S\<^isub>1 S\<^isub>2 T\<^isub>1 T\<^isub>2 x. 
+  \<lbrakk>X\<sharp>x; X\<sharp>(\<Gamma>,S\<^isub>1,T\<^isub>1); \<Gamma> \<turnstile> T\<^isub>1 <: S\<^isub>1; \<And>z. P z \<Gamma> T\<^isub>1 S\<^isub>1; ((X,T\<^isub>1)#\<Gamma>) \<turnstile> S\<^isub>2 <: T\<^isub>2; \<And>z. P z ((X,T\<^isub>1)#\<Gamma>) S\<^isub>2 T\<^isub>2\<rbrakk>
+  \<Longrightarrow> P x \<Gamma> (\<forall>[X<:S\<^isub>1].S\<^isub>2) (\<forall>[X<:T\<^isub>1].T\<^isub>2)"
   shows "P x \<Gamma> S T"
 proof -
   from a have "\<And>(pi::tyvrs prm) (x::'a::fs_tyvrs). P x (pi\<bullet>\<Gamma>) (pi\<bullet>S) (pi\<bullet>T)"
@@ -366,9 +374,6 @@ proof -
     thus "P x (pi\<bullet>\<Gamma>) (pi\<bullet>S) (pi\<bullet>Top)" by (force intro: valid_eqvt closed_in_eqvt a1)
   next
     case (S_Var S T X \<Gamma>)
-    have "\<turnstile> \<Gamma> ok" by fact
-    hence "\<turnstile> (pi\<bullet>\<Gamma>) ok" by (rule valid_eqvt)
-    moreover
     have "(X,S) \<in> set \<Gamma>" by fact
     hence "pi\<bullet>(X,S)\<in>pi\<bullet>(set \<Gamma>)" by (rule pt_set_bij2[OF pt_tyvrs_inst, OF at_tyvrs_inst])
     hence "(pi\<bullet>X,pi\<bullet>S)\<in>set (pi\<bullet>\<Gamma>)" by (simp add: pt_list_set_pi[OF pt_tyvrs_inst])
@@ -392,7 +397,7 @@ proof -
   next
     case S_Arrow thus ?case by (auto intro: a4 subtype_eqvt)
   next
-    case (S_All S1 S2 T1 T2 X \<Gamma>)
+    case (S_Forall S1 S2 T1 T2 X \<Gamma>)
     have b1: "\<Gamma> \<turnstile> T1 <: S1" by fact 
     have b2: "\<And>(pi::tyvrs prm) x. P x (pi\<bullet>\<Gamma>) (pi\<bullet>T1) (pi\<bullet>S1)" by fact
     have b4: "((X,T1)#\<Gamma>) \<turnstile> S2 <: T2" by fact
@@ -444,7 +449,7 @@ proof -
   thus ?thesis by simp
 qed
 
-subsection {* Reflexivity of Subtyping *}
+section {* Reflexivity of Subtyping *}
 
 lemma subtype_reflexivity:
   assumes a: "\<turnstile> \<Gamma> ok"
@@ -456,19 +461,20 @@ proof(nominal_induct T avoiding: \<Gamma> rule: ty.induct_unsafe)
   have ih_T\<^isub>1: "\<And>\<Gamma>. \<turnstile> \<Gamma> ok \<Longrightarrow> T\<^isub>1 closed_in \<Gamma> \<Longrightarrow> \<Gamma> \<turnstile> T\<^isub>1 <: T\<^isub>1" by fact 
   have ih_T\<^isub>2: "\<And>\<Gamma>. \<turnstile> \<Gamma> ok \<Longrightarrow> T\<^isub>2 closed_in \<Gamma> \<Longrightarrow> \<Gamma> \<turnstile> T\<^isub>2 <: T\<^isub>2" by fact
   have fresh_cond: "X\<sharp>\<Gamma>" by fact
+  hence fresh_domain: "X\<sharp>(domain \<Gamma>)" by (simp add: fresh_domain)
   have "(\<forall>[X<:T\<^isub>2].T\<^isub>1) closed_in \<Gamma>" by fact
   hence closed\<^isub>T\<^isub>2: "T\<^isub>2 closed_in \<Gamma>" and closed\<^isub>T\<^isub>1: "T\<^isub>1 closed_in ((X,T\<^isub>2)#\<Gamma>)" 
     by (auto simp add: closed_in_def ty.supp abs_supp)
   have ok: "\<turnstile> \<Gamma> ok" by fact  
-  hence ok': "\<turnstile> ((X,T\<^isub>2)#\<Gamma>) ok" using closed\<^isub>T\<^isub>2 fresh_cond by force
+  hence ok': "\<turnstile> ((X,T\<^isub>2)#\<Gamma>) ok" using closed\<^isub>T\<^isub>2 fresh_domain by simp
   have "\<Gamma> \<turnstile> T\<^isub>2 <: T\<^isub>2" using ih_T\<^isub>2 closed\<^isub>T\<^isub>2 ok by simp
   moreover
   have "((X,T\<^isub>2)#\<Gamma>) \<turnstile> T\<^isub>1 <: T\<^isub>1" using ih_T\<^isub>1 closed\<^isub>T\<^isub>1 ok' by simp
   ultimately show "\<Gamma> \<turnstile> \<forall>[X<:T\<^isub>2].T\<^isub>1 <: \<forall>[X<:T\<^isub>2].T\<^isub>1" using fresh_cond 
-    by (simp add: subtype_of.S_All)
+    by (simp add: subtype_of.S_Forall)
 qed (auto simp add: closed_in_def ty.supp supp_atm)
 
-lemma subtype_reflexivity:
+lemma subtype_reflexivity_semiautomated:
   assumes a: "\<turnstile> \<Gamma> ok"
   and     b: "T closed_in \<Gamma>"
   shows "\<Gamma> \<turnstile> T <: T"
@@ -476,10 +482,10 @@ using a b
 apply(nominal_induct T avoiding: \<Gamma> rule: ty.induct_unsafe)
 apply(auto simp add: ty.supp abs_supp closed_in_def supp_atm)
   --{* Too bad that this instantiation cannot be found automatically by
-  auto; blast cannot be used since the simplification rule 
-  @{text "closed_in_def"} needs to be applied. *}
+  \isakeyword{auto}; \isakeyword{blast} would find it if we had not used 
+  the definition @{text "closed_in_def"}. *}
 apply(drule_tac x="(tyvrs, ty2)#\<Gamma>" in meta_spec)
-apply(force simp add: closed_in_def)
+apply(force simp add: closed_in_def fresh_domain)
 done
 
 text {* Inversion lemmas *}
@@ -493,7 +499,7 @@ lemma S_ArrowE_left:
   shows "T = Top \<or> (\<exists>T1 T2. T = T1 \<rightarrow> T2 \<and> \<Gamma> \<turnstile> T1 <: S1 \<and> \<Gamma> \<turnstile> S2 <: T2)"
 using a by (cases, auto simp add: ty.inject)
 
-lemma S_AllE_left:
+lemma S_ForallE_left:
   shows "\<lbrakk>\<Gamma> \<turnstile> \<forall>[X<:S1].S2 <: T; X\<sharp>\<Gamma>; X\<sharp>S1\<rbrakk>
          \<Longrightarrow> T = Top \<or> (\<exists>T1 T2. T = \<forall>[X<:T1].T2 \<and> \<Gamma> \<turnstile> T1 <: S1 \<and> ((X,T1)#\<Gamma>) \<turnstile> S2 <: T2)"
   apply(frule subtype_implies_ok)
@@ -512,7 +518,7 @@ lemma S_AllE_left:
   apply(simp add: pt_fresh_left[OF pt_tyvrs_inst, OF at_tyvrs_inst] calc_atm)
   apply(drule_tac \<Gamma>="((Xa,T\<^isub>1)#\<Gamma>)" in  subtype_implies_closed)+
   apply(simp add: closed_in_def)
-  apply(simp add: domain_fresh[of "\<Gamma>" "X", symmetric])
+  apply(drule fresh_domain)+
   apply(simp add: fresh_def)
   apply(subgoal_tac "X \<notin> (insert Xa (domain \<Gamma>))")(*A*)
   apply(force)
@@ -534,7 +540,7 @@ section {* Type Substitution *}
 lemma subst_ty_fresh:
   fixes X :: "tyvrs"
   assumes a: "X\<sharp>(T,P)"
-  shows "X\<sharp>(subst_ty T Y P)"
+  shows "X\<sharp>T[Y:=P]\<^isub>t\<^isub>y"
   using a
   apply (nominal_induct T avoiding : T Y P rule: ty.induct_unsafe)
   apply (auto simp add: fresh_prod abs_fresh)
@@ -543,7 +549,7 @@ lemma subst_ty_fresh:
 lemma subst_ctxt_fresh:
   fixes X::"tyvrs"
   assumes a: "X\<sharp>(\<Gamma>,P)"
-  shows "X\<sharp>(subst_ctxt \<Gamma> Y P)"
+  shows "X\<sharp>\<Gamma>[Y:=P]\<^isub>t\<^isub>y\<^isub>c"
   using a
   apply (induct \<Gamma>)
   apply (auto intro: subst_ty_fresh simp add: fresh_prod fresh_list_cons)
@@ -663,8 +669,9 @@ next
 next 
   case (S_Arrow \<Gamma> S\<^isub>1 S\<^isub>2 T\<^isub>1 T\<^isub>2) thus "\<Delta> \<turnstile> S\<^isub>1 \<rightarrow> S\<^isub>2 <: T\<^isub>1 \<rightarrow> T\<^isub>2" by blast
 next
-  case (S_All \<Gamma> X S\<^isub>1 S\<^isub>2 T\<^isub>1 T\<^isub>2)
+  case (S_Forall \<Gamma> X S\<^isub>1 S\<^isub>2 T\<^isub>1 T\<^isub>2)
   have fresh_cond: "X\<sharp>\<Delta>" by fact
+  hence fresh_domain: "X\<sharp>(domain \<Delta>)" by (simp add: fresh_domain)
   have ih\<^isub>1: "\<And>\<Delta>. \<turnstile> \<Delta> ok \<Longrightarrow> \<Delta> extends \<Gamma> \<Longrightarrow> \<Delta> \<turnstile> T\<^isub>1 <: S\<^isub>1" by fact
   have ih\<^isub>2: "\<And>\<Delta>. \<turnstile> \<Delta> ok \<Longrightarrow> \<Delta> extends ((X,T\<^isub>1)#\<Gamma>) \<Longrightarrow> \<Delta> \<turnstile> S\<^isub>2 <: T\<^isub>2" by fact
   have lh_drv_prem: "\<Gamma> \<turnstile> T\<^isub>1 <: S\<^isub>1" by fact
@@ -672,26 +679,27 @@ next
   have ok: "\<turnstile> \<Delta> ok" by fact
   have ext: "\<Delta> extends \<Gamma>" by fact
   have "T\<^isub>1 closed_in \<Delta>" using ext closed\<^isub>T\<^isub>1 by (simp only: extends_closed)
-  hence "\<turnstile> ((X,T\<^isub>1)#\<Delta>) ok" using fresh_cond ok by force   
+  hence "\<turnstile> ((X,T\<^isub>1)#\<Delta>) ok" using fresh_domain ok by force   
   moreover 
   have "((X,T\<^isub>1)#\<Delta>) extends ((X,T\<^isub>1)#\<Gamma>)" using ext by (force simp add: extends_def)
   ultimately have "((X,T\<^isub>1)#\<Delta>) \<turnstile> S\<^isub>2 <: T\<^isub>2" using ih\<^isub>2 by simp
   moreover
   have "\<Delta> \<turnstile> T\<^isub>1 <: S\<^isub>1" using ok ext ih\<^isub>1 by simp 
-  ultimately show "\<Delta> \<turnstile> \<forall>[X<:S\<^isub>1].S\<^isub>2 <: \<forall>[X<:T\<^isub>1].T\<^isub>2" using ok by (force intro: S_All)
+  ultimately show "\<Delta> \<turnstile> \<forall>[X<:S\<^isub>1].S\<^isub>2 <: \<forall>[X<:T\<^isub>1].T\<^isub>2" using ok by (force intro: S_Forall)
 qed
 
 text {* In fact all "non-binding" cases can be solved automatically: *}
 
-lemma weakening:
+lemma weakening_semiautomated:
   assumes a: "\<Gamma> \<turnstile> S <: T"
   and b: "\<turnstile> \<Delta> ok"
   and c: "\<Delta> extends \<Gamma>"
   shows "\<Delta> \<turnstile> S <: T"
   using a b c 
 proof (nominal_induct \<Gamma> S T avoiding: \<Delta> rule: subtype_of_induct)
-  case (S_All \<Gamma> X S\<^isub>1 S\<^isub>2 T\<^isub>1 T\<^isub>2)
+  case (S_Forall \<Gamma> X S\<^isub>1 S\<^isub>2 T\<^isub>1 T\<^isub>2)
   have fresh_cond: "X\<sharp>\<Delta>" by fact
+  hence fresh_domain: "X\<sharp>(domain \<Delta>)" by (simp add: fresh_domain)
   have ih\<^isub>1: "\<And>\<Delta>. \<turnstile> \<Delta> ok \<Longrightarrow> \<Delta> extends \<Gamma> \<Longrightarrow> \<Delta> \<turnstile> T\<^isub>1 <: S\<^isub>1" by fact
   have ih\<^isub>2: "\<And>\<Delta>. \<turnstile> \<Delta> ok \<Longrightarrow> \<Delta> extends ((X,T\<^isub>1)#\<Gamma>) \<Longrightarrow> \<Delta> \<turnstile> S\<^isub>2 <: T\<^isub>2" by fact
   have lh_drv_prem: "\<Gamma> \<turnstile> T\<^isub>1 <: S\<^isub>1" by fact
@@ -699,230 +707,303 @@ proof (nominal_induct \<Gamma> S T avoiding: \<Delta> rule: subtype_of_induct)
   have ok: "\<turnstile> \<Delta> ok" by fact
   have ext: "\<Delta> extends \<Gamma>" by fact
   have "T\<^isub>1 closed_in \<Delta>" using ext closed\<^isub>T\<^isub>1 by (simp only: extends_closed)
-  hence "\<turnstile> ((X,T\<^isub>1)#\<Delta>) ok" using fresh_cond ok by force   
+  hence "\<turnstile> ((X,T\<^isub>1)#\<Delta>) ok" using fresh_domain ok by force   
   moreover 
   have "((X,T\<^isub>1)#\<Delta>) extends ((X,T\<^isub>1)#\<Gamma>)" using ext by (force simp add: extends_def)
   ultimately have "((X,T\<^isub>1)#\<Delta>) \<turnstile> S\<^isub>2 <: T\<^isub>2" using ih\<^isub>2 by simp
   moreover
   have "\<Delta> \<turnstile> T\<^isub>1 <: S\<^isub>1" using ok ext ih\<^isub>1 by simp 
-  ultimately show "\<Delta> \<turnstile> \<forall>[X<:S\<^isub>1].S\<^isub>2 <: \<forall>[X<:T\<^isub>1].T\<^isub>2" using ok by (force intro: S_All)
+  ultimately show "\<Delta> \<turnstile> \<forall>[X<:S\<^isub>1].S\<^isub>2 <: \<forall>[X<:T\<^isub>1].T\<^isub>2" using ok by (force intro: S_Forall)
 qed (blast intro: extends_closed extends_memb dest: extends_domain)+
 
-text {* our contexts grow from right to left *}
+text {* Next we prove the transitivity and narrowing for the subtyping relation. 
+The POPLmark-paper says the following:
 
-lemma transitivity_and_narrowing:
-  shows "\<Gamma> \<turnstile> S <: Q \<Longrightarrow> \<Gamma> \<turnstile> Q <: T \<Longrightarrow> \<Gamma> \<turnstile> S <: T"
-  and "(\<Delta>@[(X,Q)]@\<Gamma>) \<turnstile> M <: N \<Longrightarrow> \<Gamma> \<turnstile> P <: Q \<Longrightarrow> (\<Delta>@[(X,P)]@\<Gamma>) \<turnstile> M <: N"
-proof (induct Q fixing: \<Gamma> S T and \<Delta> \<Gamma> X P M N taking: "size_ty" rule: measure_induct_rule)
-  case (less Q) 
-  note IH_trans = prems[THEN conjunct1, rule_format]
-  note IH_narrow = prems[THEN conjunct2, THEN spec, of _ "[]", simplified, rule_format]
+\begin{lemma}[Transitivity and Narrowing] \
+\begin{enumerate}
+\item If @{term "\<Gamma> \<turnstile> S<:Q"} and @{term "\<Gamma> \<turnstile> Q<:T"}, then @{term "\<Gamma> \<turnstile> S<:T"}.
+\item If @{text "\<Gamma>,X<:Q,\<Delta> \<turnstile> M<:N"} and @{term "\<Gamma> \<turnstile> P<:Q"} then @{text "\<Gamma>,X<:P,\<Delta> \<turnstile> M<:N"}.
+\end{enumerate}
+\end{lemma}
 
-    --{* The inner induction for transitivity over @{term "\<Gamma> \<turnstile> S <: Q"} *}
-  have transitivity: 
-    "\<And>\<Gamma> S T. \<Gamma> \<turnstile> S <: Q \<Longrightarrow> \<Gamma> \<turnstile> Q <: T \<Longrightarrow> \<Gamma> \<turnstile> S <: T"
+The two parts are proved simultaneously, by induction on the size
+of @{term "Q"}.  The argument for part (2) assumes that part (1) has 
+been established already for the @{term "Q"} in question; part (1) uses 
+part (2) only for strictly smaller @{term "Q"}.
+
+For the induction on the size of @{term "Q"}, we use the induction-rule 
+@{text "measure_induct_rule"}:
+
+\begin{center}
+@{thm measure_induct_rule[of "size_ty",no_vars]}
+\end{center}
+
+It says in English: in order to show a property @{term "P a"} for all @{term "a"}, 
+it requires to prove that for all @{term x} @{term "P x"} holds using the 
+assumption that for all @{term y} whose size is strictly smaller than 
+that of @{term x} the property @{term "P y"} holds. *}
+
+lemma 
+  shows trans: "\<Gamma>\<turnstile>S<:Q \<Longrightarrow> \<Gamma>\<turnstile>Q<:T \<Longrightarrow> \<Gamma>\<turnstile>S<:T" 
+  and narrow: "(\<Delta>@[(X,Q)]@\<Gamma>)\<turnstile>M<:N \<Longrightarrow> \<Gamma>\<turnstile>P<:Q \<Longrightarrow> (\<Delta>@[(X,P)]@\<Gamma>)\<turnstile>M<:N"
+proof (induct Q fixing: \<Gamma> S T \<Delta> X P M N taking: "size_ty" rule: measure_induct_rule)
+  case (less Q)
+    --{* \begin{minipage}[t]{0.9\textwidth}
+    First we mention the induction hypotheses of the outer induction for later
+    reference:\end{minipage}*}
+  have IH_trans:  
+    "\<And>Q' \<Gamma> S T. \<lbrakk>size_ty Q' < size_ty Q; \<Gamma>\<turnstile>S<:Q'; \<Gamma>\<turnstile>Q'<:T\<rbrakk> \<Longrightarrow> \<Gamma>\<turnstile>S<:T" by fact
+  have IH_narrow:
+    "\<And>Q' \<Delta> \<Gamma> X M N P. \<lbrakk>size_ty Q' < size_ty Q; (\<Delta>@[(X,Q')]@\<Gamma>)\<turnstile>M<:N; \<Gamma>\<turnstile>P<:Q'\<rbrakk> 
+    \<Longrightarrow> (\<Delta>@[(X,P)]@\<Gamma>)\<turnstile>M<:N" by fact
+    --{* \begin{minipage}[t]{0.9\textwidth}
+    We proceed with the transitivity proof as an auxiliary lemma, because it needs 
+    to be referenced in the narrowing proof.\end{minipage}*}
+  have transitivity_aux:
+    "\<And>\<Gamma> S T. \<lbrakk>\<Gamma> \<turnstile> S <: Q; \<Gamma> \<turnstile> Q <: T\<rbrakk> \<Longrightarrow> \<Gamma> \<turnstile> S <: T"
   proof - 
-    
-      -- {* We first handle the case where T = Top once and for all; this saves some 
-      repeated argument below (just like on paper :-).  To do so we establish a little 
-      lemma that is invoked where needed in the induction for transitivity. *} 
-    have top_case: 
-      "\<And>\<Gamma> S T' P. \<lbrakk>\<turnstile> \<Gamma> ok; S closed_in \<Gamma>; P \<Longrightarrow> \<Gamma> \<turnstile> S <: T'; T'=Top \<or> P\<rbrakk> \<Longrightarrow> \<Gamma> \<turnstile> S <: T'"
-    proof - 
-      fix \<Gamma> S T' P
-      assume S_Top_prm1: "S closed_in \<Gamma>"
-	and  S_Top_prm2: "\<turnstile> \<Gamma> ok"
-	and  alternative: "P \<Longrightarrow> \<Gamma> \<turnstile> S <: T'" 
-	and  "T'=Top \<or> P" 
-      moreover
-      { assume "T'=Top"
-	hence "\<Gamma> \<turnstile> S <: T'" using S_Top_prm1 S_Top_prm2 by (simp add: S_Top)
-      } 
-      moreover 
-      { assume P 
-	with alternative have "\<Gamma> \<turnstile> S <: T'" by simp 
-      }
-      ultimately show "\<Gamma> \<turnstile> S <: T'" by blast
-    qed
-
-	--{* Now proceed by the inner induction on the left-hand derivation *}
     fix \<Gamma>' S' T
-    assume a: "\<Gamma>' \<turnstile> S' <: Q" --{* lh derivation *}
-    assume b: "\<Gamma>' \<turnstile> Q <: T" --{* rh derivation *}
-    from a b show "\<Gamma>' \<turnstile> S' <: T"
-    proof(nominal_induct \<Gamma>' S' Q\<equiv>Q avoiding: \<Gamma>' S' T rule: subtype_of_induct)
+    assume "\<Gamma>' \<turnstile> S' <: Q" --{* left-hand derivation *}
+      and  "\<Gamma>' \<turnstile> Q <: T"  --{* right-hand derivation *}
+    thus "\<Gamma>' \<turnstile> S' <: T"
+    proof (nominal_induct \<Gamma>' S' Q\<equiv>Q avoiding: \<Gamma>' S' rule: subtype_of_induct) 
       case (S_Top \<Gamma> S) 
-	--{* in this case lh drv is @{term "\<Gamma> \<turnstile> S <: Top"} *}
+	--{* \begin{minipage}[t]{0.9\textwidth}
+	In this case the left-hand derivation is @{term "\<Gamma> \<turnstile> S <: Top"}, giving
+	us @{term "\<turnstile> \<Gamma> ok"} and @{term "S closed_in \<Gamma>"}. This case is straightforward, 
+	because the right-hand derivation must be of the form @{term "\<Gamma> \<turnstile> Top <: Top"} 
+	giving us the equation @{term "T = Top"}.\end{minipage}*}
       hence rh_drv: "\<Gamma> \<turnstile> Top <: T" by simp
       hence T_inst: "T = Top" by (simp add: S_TopE)
-      have lh_drv_prm1: "\<turnstile> \<Gamma> ok" by fact
-      have lh_drv_prm2: "S closed_in \<Gamma>" by fact
-      from lh_drv_prm1 lh_drv_prm2 have "\<Gamma> \<turnstile> S <: Top" by (simp add: subtype_of.S_Top)
+      have "\<turnstile> \<Gamma> ok" 
+	and "S closed_in \<Gamma>" by fact
+      hence "\<Gamma> \<turnstile> S <: Top" by (simp add: subtype_of.S_Top)
       thus "\<Gamma> \<turnstile> S <: T" using T_inst by simp
     next
-      case (S_Var \<Gamma> Y U Q) 
-	--{* in this case lh drv is @{term "\<Gamma> \<turnstile> Tvar(Y) <: Q"} *}
+      case (S_Var \<Gamma> Y U) 
+	-- {* \begin{minipage}[t]{0.9\textwidth}
+	In this case the left-hand derivation is @{term "\<Gamma> \<turnstile> Tvar Y <: Q"} 
+	with @{term "S = Tvar Y"}. We have therefore @{term "(Y,U)"} 
+	is in @{term "\<Gamma>"} and by inner induction hypothesis @{term "\<Gamma> \<turnstile> U <: T"}. 
+	By @{text "S_Var"} follows @{term "\<Gamma> \<turnstile> Tvar Y <: T"}.\end{minipage}*}
       hence IH_inner: "\<Gamma> \<turnstile> U <: T" by simp
-      have lh_drv_prm1: "\<turnstile> \<Gamma> ok" by fact
-      have lh_drv_prm2: "(Y,U)\<in>set \<Gamma>" by fact
-      from IH_inner show "\<Gamma> \<turnstile> Tvar Y <: T" using lh_drv_prm1 lh_drv_prm2 
-	by (simp add: subtype_of.S_Var)
+      have "(Y,U) \<in> set \<Gamma>" by fact
+      with IH_inner show "\<Gamma> \<turnstile> Tvar Y <: T" by (simp add: subtype_of.S_Var)
     next
       case (S_Refl \<Gamma> X) 
-	--{* in this case lh drv is @{term "\<Gamma> \<turnstile> Tvar X <: Tvar X"} *}
+	--{* \begin{minipage}[t]{0.9\textwidth}
+        In this case the left-hand derivation is @{term "\<Gamma>\<turnstile>(Tvar X) <: (Tvar X)"} with
+        @{term "Q=Tvar X"}. The goal then follows immediately from the right-hand 
+	derivation.\end{minipage}*}
       thus "\<Gamma> \<turnstile> Tvar X <: T" by simp
     next
-      case (S_Arrow \<Gamma> S1 S2 Q1 Q2) 
-	--{* in this case lh drv is @{term "\<Gamma> \<turnstile> S1 \<rightarrow> S2 <: Q1 \<rightarrow> Q2"} *}
-      hence rh_drv: "\<Gamma> \<turnstile> Q1 \<rightarrow> Q2 <: T" by simp
-      have Q_inst: "Q1 \<rightarrow> Q2 = Q" by fact
-      hence Q1_less: "size_ty Q1 < size_ty Q" 
-	and Q2_less: "size_ty Q2 < size_ty Q" by auto
-      have lh_drv_prm1: "\<Gamma> \<turnstile> Q1 <: S1" by fact
-      have lh_drv_prm2: "\<Gamma> \<turnstile> S2 <: Q2" by fact      
-      have "S1 closed_in \<Gamma>" and "S2 closed_in \<Gamma>" 
-	using lh_drv_prm1 lh_drv_prm2 by (simp_all add: subtype_implies_closed)
-      hence "(S1 \<rightarrow> S2) closed_in \<Gamma>" by (simp add: closed_in_def ty.supp)
-      moreover
-      have "\<turnstile> \<Gamma> ok" using rh_drv by (rule subtype_implies_ok)
-      moreover
-      from rh_drv have "T = Top \<or> (\<exists>T1 T2.  T = T1 \<rightarrow> T2 \<and> \<Gamma> \<turnstile> T1 <: Q1 \<and> \<Gamma> \<turnstile> Q2 <: T2)" 
+      case (S_Arrow \<Gamma> S\<^isub>1 S\<^isub>2 Q\<^isub>1 Q\<^isub>2) 
+	--{* \begin{minipage}[t]{0.9\textwidth}
+	In this case the left-hand derivation is @{term "\<Gamma> \<turnstile> S\<^isub>1 \<rightarrow> S\<^isub>2 <: Q\<^isub>1 \<rightarrow> Q\<^isub>2"} with
+        @{term "S\<^isub>1\<rightarrow>S\<^isub>2=S"} and @{term "Q\<^isub>1\<rightarrow>Q\<^isub>2=Q"}. We know that the @{text "size_ty"} of 
+	@{term Q\<^isub>1} and @{term Q\<^isub>2} is smaller than that of @{term Q};
+	so we can apply the outer induction hypotheses for @{term Q\<^isub>1} and @{term Q\<^isub>2}. 
+	We also have the sub-derivations  @{term "\<Gamma>\<turnstile>Q\<^isub>1<:S\<^isub>1"} and @{term "\<Gamma>\<turnstile>S\<^isub>2<:Q\<^isub>2"}.
+	The right-hand derivation is @{term "\<Gamma> \<turnstile> Q\<^isub>1 \<rightarrow> Q\<^isub>2 <: T"}. There exists types 
+	@{text "T\<^isub>1,T\<^isub>2"} such that @{term "T=Top \<or> T=T\<^isub>1\<rightarrow>T\<^isub>2"}. The @{term "Top"}-case is 
+	straightforward once we know @{term "(S\<^isub>1 \<rightarrow> S\<^isub>2) closed_in \<Gamma>"} and @{term "\<turnstile> \<Gamma> ok"}. 
+	In the other case we have the sub-derivations @{term "\<Gamma>\<turnstile>T\<^isub>1<:Q\<^isub>1"} and @{term "\<Gamma>\<turnstile>Q\<^isub>2<:T\<^isub>2"}. 
+	Using the outer induction hypothesis for transitivity we can derive @{term "\<Gamma>\<turnstile>T\<^isub>1<:S\<^isub>1"} 
+	and @{term "\<Gamma>\<turnstile>S\<^isub>2<:T\<^isub>2"}. By rule @{text "S_Arrow"} follows @{term "\<Gamma> \<turnstile> S\<^isub>1 \<rightarrow> S\<^isub>2 <: T\<^isub>1 \<rightarrow> T\<^isub>2"},
+	which is @{term "\<Gamma> \<turnstile> S\<^isub>1 \<rightarrow> S\<^isub>2 <: T\<^isub>"}.\end{minipage}*}
+      hence rh_drv: "\<Gamma> \<turnstile> Q\<^isub>1 \<rightarrow> Q\<^isub>2 <: T" by simp
+      from `Q\<^isub>1 \<rightarrow> Q\<^isub>2 = Q` 
+      have Q\<^isub>1\<^isub>2_less: "size_ty Q\<^isub>1 < size_ty Q" "size_ty Q\<^isub>2 < size_ty Q" by auto
+      have lh_drv_prm\<^isub>1: "\<Gamma> \<turnstile> Q\<^isub>1 <: S\<^isub>1" by fact
+      have lh_drv_prm\<^isub>2: "\<Gamma> \<turnstile> S\<^isub>2 <: Q\<^isub>2" by fact      
+      from rh_drv have "T=Top \<or> (\<exists>T\<^isub>1 T\<^isub>2. T=T\<^isub>1\<rightarrow>T\<^isub>2 \<and> \<Gamma>\<turnstile>T\<^isub>1<:Q\<^isub>1 \<and> \<Gamma>\<turnstile>Q\<^isub>2<:T\<^isub>2)" 
 	by (simp add: S_ArrowE_left)  
       moreover
-      { assume "\<exists>T1 T2. T = T1 \<rightarrow> T2 \<and> \<Gamma> \<turnstile> T1 <: Q1 \<and> \<Gamma> \<turnstile> Q2 <: T2"
-	then obtain T1 T2 
-	  where T_inst: "T = T1 \<rightarrow> T2" 
-	  and   rh_drv_prm1: "\<Gamma> \<turnstile> T1 <: Q1"
-	  and   rh_drv_prm2: "\<Gamma> \<turnstile> Q2 <: T2" by force
-        from IH_trans[of "Q1"] have "\<Gamma> \<turnstile> T1 <: S1" using Q1_less rh_drv_prm1 lh_drv_prm1 by simp 
-	moreover
-	from IH_trans[of "Q2"] have "\<Gamma> \<turnstile> S2 <: T2" using Q2_less rh_drv_prm2 lh_drv_prm2 by simp
-	ultimately have "\<Gamma> \<turnstile> S1 \<rightarrow> S2 <: T1 \<rightarrow> T2" by (simp add: subtype_of.S_Arrow)
-	hence "\<Gamma> \<turnstile> S1 \<rightarrow> S2 <: T" using T_inst by simp
-      }
-      ultimately show "\<Gamma> \<turnstile> S1 \<rightarrow> S2 <: T" using top_case by blast
-    next
-      case (S_All \<Gamma> X S1 S2 Q1 Q2) 
-	--{* in this case lh drv is @{term "\<Gamma>\<turnstile>\<forall>[X<:S1].S2 <: \<forall>[X<:Q1].Q2"} *}
-      hence rh_drv: "\<Gamma> \<turnstile> \<forall>[X<:Q1].Q2 <: T" by simp
-      have lh_drv_prm1: "\<Gamma> \<turnstile> Q1 <: S1" by fact
-      have lh_drv_prm2: "((X,Q1)#\<Gamma>) \<turnstile> S2 <: Q2" by fact
-      have fresh_cond: "X\<sharp>\<Gamma>" "X\<sharp>Q1" by fact
-      have Q_inst: "\<forall>[X<:Q1].Q2 = Q" by fact
-      hence Q1_less: "size_ty Q1 < size_ty Q" 
-	and Q2_less: "size_ty Q2 < size_ty Q " by auto
-      have "S1 closed_in \<Gamma>" and "S2 closed_in ((X,Q1)#\<Gamma>)" 
-	using lh_drv_prm1 lh_drv_prm2 by (simp_all add: subtype_implies_closed)
-      hence "(\<forall>[X<:S1].S2) closed_in \<Gamma>" by (force simp add: closed_in_def ty.supp abs_supp)
+      have "S\<^isub>1 closed_in \<Gamma>" and "S\<^isub>2 closed_in \<Gamma>" 
+	using lh_drv_prm\<^isub>1 lh_drv_prm\<^isub>2 by (simp_all add: subtype_implies_closed)
+      hence "(S\<^isub>1 \<rightarrow> S\<^isub>2) closed_in \<Gamma>" by (simp add: closed_in_def ty.supp)
       moreover
       have "\<turnstile> \<Gamma> ok" using rh_drv by (rule subtype_implies_ok)
       moreover
-      from rh_drv have "T = Top \<or> (\<exists>T1 T2. T = \<forall>[X<:T1].T2 \<and> \<Gamma> \<turnstile> T1 <: Q1 \<and> ((X,T1)#\<Gamma>) \<turnstile> Q2 <: T2)" 
-	using fresh_cond by (simp add: S_AllE_left)
-      moreover
-      { assume "\<exists>T1 T2. T = \<forall>[X<:T1].T2 \<and> \<Gamma> \<turnstile> T1 <: Q1 \<and> ((X,T1)#\<Gamma>) \<turnstile> Q2 <: T2"
-	then obtain T1 T2 
-	  where T_inst: "T = \<forall>[X<:T1].T2" 
-	  and   rh_drv_prm1: "\<Gamma> \<turnstile> T1 <: Q1" 
-	  and   rh_drv_prm2:"((X,T1)#\<Gamma>) \<turnstile> Q2 <: T2" by force
-        from IH_trans[of "Q1"] have "\<Gamma> \<turnstile> T1 <: S1" 
-	  using lh_drv_prm1 rh_drv_prm1 Q1_less by blast
-        moreover
-	from IH_narrow[of "Q1"] have "((X,T1)#\<Gamma>) \<turnstile> S2 <: Q2" 
-	  using Q1_less lh_drv_prm2 rh_drv_prm1 by blast
-	with IH_trans[of "Q2"] have "((X,T1)#\<Gamma>) \<turnstile> S2 <: T2" 
-	  using Q2_less rh_drv_prm2 by blast
-        moreover
-	ultimately have "\<Gamma> \<turnstile> \<forall>[X<:S1].S2 <: \<forall>[X<:T1].T2"
-	  using fresh_cond by (simp add: subtype_of.S_All)
-	hence "\<Gamma> \<turnstile> \<forall>[X<:S1].S2 <: T" using T_inst by simp
+      { assume "\<exists>T\<^isub>1 T\<^isub>2. T=T\<^isub>1\<rightarrow>T\<^isub>2 \<and> \<Gamma>\<turnstile>T\<^isub>1<:Q\<^isub>1 \<and> \<Gamma>\<turnstile>Q\<^isub>2<:T\<^isub>2"
+	then obtain T\<^isub>1 T\<^isub>2 
+	  where T_inst: "T = T\<^isub>1 \<rightarrow> T\<^isub>2" 
+	  and   rh_drv_prm\<^isub>1: "\<Gamma> \<turnstile> T\<^isub>1 <: Q\<^isub>1"
+	  and   rh_drv_prm\<^isub>2: "\<Gamma> \<turnstile> Q\<^isub>2 <: T\<^isub>2" by force
+	from IH_trans[of "Q\<^isub>1"] 
+	have "\<Gamma> \<turnstile> T\<^isub>1 <: S\<^isub>1" using Q\<^isub>1\<^isub>2_less rh_drv_prm\<^isub>1 lh_drv_prm\<^isub>1 by simp 
+	moreover
+	from IH_trans[of "Q\<^isub>2"] 
+	have "\<Gamma> \<turnstile> S\<^isub>2 <: T\<^isub>2" using Q\<^isub>1\<^isub>2_less rh_drv_prm\<^isub>2 lh_drv_prm\<^isub>2 by simp
+	ultimately have "\<Gamma> \<turnstile> S\<^isub>1 \<rightarrow> S\<^isub>2 <: T\<^isub>1 \<rightarrow> T\<^isub>2" by (simp add: subtype_of.S_Arrow)
+	hence "\<Gamma> \<turnstile> S\<^isub>1 \<rightarrow> S\<^isub>2 <: T" using T_inst by simp
       }
-      ultimately show "\<Gamma> \<turnstile> \<forall>[X<:S1].S2 <: T" using top_case by blast
+      ultimately show "\<Gamma> \<turnstile> S\<^isub>1 \<rightarrow> S\<^isub>2 <: T" by blast
+    next
+      case (S_Forall \<Gamma> X S\<^isub>1 S\<^isub>2 Q\<^isub>1 Q\<^isub>2) 
+	--{* \begin{minipage}[t]{0.9\textwidth}
+	In this case the left-hand derivation is @{text "\<Gamma>\<turnstile>\<forall>[X<:S\<^isub>1].S\<^isub>2 <: \<forall>[X<:Q\<^isub>1].Q\<^isub>2"} with 
+	@{text "\<forall>[X<:S\<^isub>1].S\<^isub>2=S"} and @{text "\<forall>[X<:Q\<^isub>1].Q\<^isub>2=Q"}. We therefore have the sub-derivations  
+	@{term "\<Gamma>\<turnstile>Q\<^isub>1<:S\<^isub>1"} and @{term "((X,Q\<^isub>1)#\<Gamma>)\<turnstile>S\<^isub>2<:Q\<^isub>2"}. Since @{term "X"} is a binder, we
+	assume that it is sufficiently fresh; in particular we have the freshness conditions
+	@{term "X\<sharp>\<Gamma>"} and @{term "X\<sharp>Q\<^isub>1"} (these assumptions are provided by the strong induction
+	rule @{text "subtype_of_induct"}). We know that the @{text "size_ty"} of 
+	@{term Q\<^isub>1} and @{term Q\<^isub>2} is smaller than that of @{term Q};
+	so we can apply the outer induction hypotheses for @{term Q\<^isub>1} and @{term Q\<^isub>2}. 
+	The right-hand derivation is @{text "\<Gamma> \<turnstile> \<forall>[X<:Q\<^isub>1].Q\<^isub>2 <: T"}. Since @{term "X\<sharp>\<Gamma>"} 
+	and @{term "X\<sharp>Q\<^isub>1"} there exists types @{text "T\<^isub>1,T\<^isub>2"} such that 
+	@{text "T=Top \<or> T=\<forall>[X<:T\<^isub>1].T\<^isub>2"}. The @{term "Top"}-case is straightforward once we know 
+	@{text "(\<forall>[X<:S\<^isub>1].S\<^isub>2) closed_in \<Gamma>"} and @{term "\<turnstile> \<Gamma> ok"}. In the other case we have 
+	the sub-derivations @{term "\<Gamma>\<turnstile>T\<^isub>1<:Q\<^isub>1"}. @{term "((X,T\<^isub>1)#\<Gamma>)\<turnstile>Q\<^isub>2<:T\<^isub>2"}. Using the outer 
+	induction hypothesis for transitivity we can derive @{term "\<Gamma>\<turnstile>T\<^isub>1<:S\<^isub>1"}. From the outer 
+	induction for narrowing we get @{term "((X,T\<^isub>1)#\<Gamma>) \<turnstile> S\<^isub>2 <: Q\<^isub>2"} and then using induction 
+	again @{term "((X,T\<^isub>1)#\<Gamma>) \<turnstile> S\<^isub>2 <: T\<^isub>2"}. By rule @{text "S_Forall"} and the freshness 
+	condition @{term "X\<sharp>\<Gamma>"} follows @{text "\<Gamma> \<turnstile> \<forall>[X<:S\<^isub>1].S\<^isub>2 <: \<forall>[X<:T\<^isub>1].T\<^isub>2"}.which is 
+	@{text "\<Gamma> \<turnstile>  \<forall>[X<:S\<^isub>1].S\<^isub>2 <: T\<^isub>"}.\end{minipage}*}
+      hence rh_drv: "\<Gamma> \<turnstile> \<forall>[X<:Q\<^isub>1].Q\<^isub>2 <: T" by simp
+      have lh_drv_prm\<^isub>1: "\<Gamma> \<turnstile> Q\<^isub>1 <: S\<^isub>1" by fact
+      have lh_drv_prm\<^isub>2: "((X,Q\<^isub>1)#\<Gamma>) \<turnstile> S\<^isub>2 <: Q\<^isub>2" by fact
+      have fresh_cond: "X\<sharp>\<Gamma>" "X\<sharp>Q\<^isub>1" by fact
+      from `\<forall>[X<:Q\<^isub>1].Q\<^isub>2 = Q` 
+      have Q\<^isub>1\<^isub>2_less: "size_ty Q\<^isub>1 < size_ty Q" "size_ty Q\<^isub>2 < size_ty Q " by auto
+      from rh_drv 
+      have "T=Top \<or> (\<exists>T\<^isub>1 T\<^isub>2. T=\<forall>[X<:T\<^isub>1].T\<^isub>2 \<and> \<Gamma>\<turnstile>T\<^isub>1<:Q\<^isub>1 \<and> ((X,T\<^isub>1)#\<Gamma>)\<turnstile>Q\<^isub>2<:T\<^isub>2)" 
+	using fresh_cond by (simp add: S_ForallE_left)
+      moreover
+      have "S\<^isub>1 closed_in \<Gamma>" and "S\<^isub>2 closed_in ((X,Q\<^isub>1)#\<Gamma>)" 
+	using lh_drv_prm\<^isub>1 lh_drv_prm\<^isub>2 by (simp_all add: subtype_implies_closed)
+      hence "(\<forall>[X<:S\<^isub>1].S\<^isub>2) closed_in \<Gamma>" by (force simp add: closed_in_def ty.supp abs_supp)
+      moreover
+      have "\<turnstile> \<Gamma> ok" using rh_drv by (rule subtype_implies_ok)
+      moreover
+      { assume "\<exists>T\<^isub>1 T\<^isub>2. T=\<forall>[X<:T\<^isub>1].T\<^isub>2 \<and> \<Gamma>\<turnstile>T\<^isub>1<:Q\<^isub>1 \<and> ((X,T\<^isub>1)#\<Gamma>)\<turnstile>Q\<^isub>2<:T\<^isub>2"
+	then obtain T\<^isub>1 T\<^isub>2 
+	  where T_inst: "T = \<forall>[X<:T\<^isub>1].T\<^isub>2" 
+	  and   rh_drv_prm\<^isub>1: "\<Gamma> \<turnstile> T\<^isub>1 <: Q\<^isub>1" 
+	  and   rh_drv_prm\<^isub>2:"((X,T\<^isub>1)#\<Gamma>) \<turnstile> Q\<^isub>2 <: T\<^isub>2" by force
+	from IH_trans[of "Q\<^isub>1"] 
+	have "\<Gamma> \<turnstile> T\<^isub>1 <: S\<^isub>1" using lh_drv_prm\<^isub>1 rh_drv_prm\<^isub>1 Q\<^isub>1\<^isub>2_less by blast
+	moreover
+	from IH_narrow[of "Q\<^isub>1" "[]"] 
+	have "((X,T\<^isub>1)#\<Gamma>) \<turnstile> S\<^isub>2 <: Q\<^isub>2" using Q\<^isub>1\<^isub>2_less lh_drv_prm\<^isub>2 rh_drv_prm\<^isub>1 by simp
+	with IH_trans[of "Q\<^isub>2"] 
+	have "((X,T\<^isub>1)#\<Gamma>) \<turnstile> S\<^isub>2 <: T\<^isub>2" using Q\<^isub>1\<^isub>2_less rh_drv_prm\<^isub>2 by simp
+	ultimately have "\<Gamma> \<turnstile> \<forall>[X<:S\<^isub>1].S\<^isub>2 <: \<forall>[X<:T\<^isub>1].T\<^isub>2"
+	  using fresh_cond by (simp add: subtype_of.S_Forall)
+	hence "\<Gamma> \<turnstile> \<forall>[X<:S\<^isub>1].S\<^isub>2 <: T" using T_inst by simp
+      }
+      ultimately show "\<Gamma> \<turnstile> \<forall>[X<:S\<^isub>1].S\<^isub>2 <: T" by blast
     qed
   qed
 
-  --{* The inner induction for narrowing over @{term "(\<Delta>@[(X,Q)]@\<Gamma>) \<turnstile> M <: N"} *}
-  have narrowing:
-    "\<And>\<Delta> \<Gamma> X M N P. (\<Delta>@[(X,Q)]@\<Gamma>) \<turnstile> M <: N \<Longrightarrow> \<Gamma> \<turnstile> P<:Q \<Longrightarrow> (\<Delta>@[(X,P)]@\<Gamma>) \<turnstile> M <: N"
-  proof -
-    fix \<Delta>' \<Gamma>' X M N P
-    assume a: "(\<Delta>'@[(X,Q)]@\<Gamma>') \<turnstile> M <: N"
-    assume b: "\<Gamma>' \<turnstile> P<:Q"
-    from a b show "(\<Delta>'@[(X,P)]@\<Gamma>') \<turnstile> M <: N" 
-    proof (nominal_induct \<Gamma>\<equiv>"\<Delta>'@[(X,Q)]@\<Gamma>'" M N avoiding: \<Delta>' \<Gamma>' X rule: subtype_of_induct) 
+  { --{* The transitivity proof is now by the auxiliary lemma. *}
+    case 1 
+    have  "\<Gamma> \<turnstile> S <: Q" 
+      and "\<Gamma> \<turnstile> Q <: T" by fact
+    thus "\<Gamma> \<turnstile> S <: T" by (rule transitivity_aux) 
+  next 
+    --{* The narrowing proof proceeds by an induction over @{term "(\<Delta>@[(X,Q)]@\<Gamma>) \<turnstile> M <: N"}. *}
+    case 2
+    have  "(\<Delta>@[(X,Q)]@\<Gamma>) \<turnstile> M <: N" --{* left-hand derivation *}
+      and "\<Gamma> \<turnstile> P<:Q" by fact --{* right-hand derivation *}
+    thus "(\<Delta>@[(X,P)]@\<Gamma>) \<turnstile> M <: N" 
+    proof (nominal_induct \<Gamma>\<equiv>"\<Delta>@[(X,Q)]@\<Gamma>" M N avoiding: \<Delta> \<Gamma> X rule: subtype_of_induct) 
       case (S_Top _ S \<Delta> \<Gamma> X)
-	--{* in this case lh drv is @{term "(\<Delta>@[(X,Q)]@\<Gamma>) \<turnstile> S <: Top"} *}
-      hence lh_drv_prm1: "\<turnstile> (\<Delta>@[(X,Q)]@\<Gamma>) ok" 
-        and lh_drv_prm2: "S closed_in (\<Delta>@[(X,Q)]@\<Gamma>)" by simp_all
+	--{* \begin{minipage}[t]{0.9\textwidth}
+	In this case the left-hand derivation is @{term "(\<Delta>@[(X,Q)]@\<Gamma>) \<turnstile> S <: Top"}. We show
+	that the context @{term "\<Delta>@[(X,P)]@\<Gamma>"} is ok and that @{term S} is closed in 
+	@{term "\<Delta>@[(X,P)]@\<Gamma>"}. Then we can apply the @{text "S_Top"}-rule.\end{minipage}*}
+      hence lh_drv_prm\<^isub>1: "\<turnstile> (\<Delta>@[(X,Q)]@\<Gamma>) ok" 
+	and lh_drv_prm\<^isub>2: "S closed_in (\<Delta>@[(X,Q)]@\<Gamma>)" by simp_all
       have rh_drv: "\<Gamma> \<turnstile> P <: Q" by fact
       hence "P closed_in \<Gamma>" by (simp add: subtype_implies_closed)
-      with lh_drv_prm1 have "\<turnstile> (\<Delta>@[(X,P)]@\<Gamma>) ok" by (simp add: replace_type)
+      with lh_drv_prm\<^isub>1 have "\<turnstile> (\<Delta>@[(X,P)]@\<Gamma>) ok" by (simp add: replace_type)
       moreover
-      from lh_drv_prm2 have "S closed_in (\<Delta>@[(X,P)]@\<Gamma>)" by (simp add: closed_in_def domain_append)
+      from lh_drv_prm\<^isub>2 have "S closed_in (\<Delta>@[(X,P)]@\<Gamma>)" 
+	by (simp add: closed_in_def domain_append)
       ultimately show "(\<Delta>@[(X,P)]@\<Gamma>) \<turnstile> S <: Top" by (simp add: subtype_of.S_Top)
     next
       case (S_Var _ Y S N \<Delta> \<Gamma> X) 
-	--{* in this case lh drv is @{term "(\<Delta>@[(X,Q)]@\<Gamma>) \<turnstile> Tvar Y <: N"} *}
-      hence IH_inner: "(\<Delta>@[(X,P)]@\<Gamma>) \<turnstile> S <: N" 
-	and lh_drv_prm1: "\<turnstile> (\<Delta>@[(X,Q)]@\<Gamma>) ok" 
-        and lh_drv_prm2: "(Y,S)\<in>set (\<Delta>@[(X,Q)]@\<Gamma>)" by simp_all
-      have rh_drv: "\<Gamma> \<turnstile> P <: Q" by fact
-      hence "P closed_in \<Gamma>" by (simp add: subtype_implies_closed)
-      hence cntxt_ok: "\<turnstile> (\<Delta>@[(X,P)]@\<Gamma>) ok" using lh_drv_prm1 by (simp add: replace_type)
-	-- {* we distinguishing the cases @{term "X\<noteq>Y"} and @{term "X=Y"} (the latter 
-	being the interesting one) *}
-      { assume "X\<noteq>Y"
-	hence "(Y,S)\<in>set (\<Delta>@[(X,P)]@\<Gamma>)" using lh_drv_prm2 by simp
-	with IH_inner have "(\<Delta>@[(X,P)]@\<Gamma>) \<turnstile> Tvar Y <: N" 
-	  using cntxt_ok by (simp add: subtype_of.S_Var)
-      }
-      moreover
-      { have memb_XQ: "(X,Q)\<in>set (\<Delta>@[(X,Q)]@\<Gamma>)" by simp
-	have memb_XP: "(X,P)\<in>set (\<Delta>@[(X,P)]@\<Gamma>)" by simp
-	assume "X=Y" 
-	hence "S=Q" using lh_drv_prm1 lh_drv_prm2 memb_XQ by (simp only: uniqueness_of_ctxt)
+	--{* \begin{minipage}[t]{0.9\textwidth}
+	In this case the left-hand derivation is @{term "(\<Delta>@[(X,Q)]@\<Gamma>) \<turnstile> Tvar Y <: N"}. We therefore 
+	know that the contexts @{term "\<Delta>@[(X,Q)]@\<Gamma>"} and @{term "\<Delta>@[(X,P)]@\<Gamma>"} are ok, and that 
+	@{term "(Y,S)"} is in @{term "\<Delta>@[(X,Q)]@\<Gamma>"}. By inner induction hypothesis we have 
+	@{term "(\<Delta>@[(X,P)]@\<Gamma>) \<turnstile> S <: N"}. We need to show that @{term "(\<Delta>@[(X,P)]@\<Gamma>) \<turnstile> Tvar Y <: N"} 
+	holds. In case @{term "X\<noteq>Y"} we know that @{term "(Y,S)"} is in @{term "\<Delta>@[(X,P)]@\<Gamma>"} and 
+	can use the inner induction hypothesis and rule @{text "S_Var"} to conclude. In case 
+	@{term "X=Y"} we can infer that @{term "S=Q"}; moreover we have that 
+	@{term "(\<Delta>@[(X,P)]@\<Gamma>) extends \<Gamma>"} and therefore by @{text "weakening"} that 
+	@{term "(\<Delta>@[(X,P)]@\<Gamma>) \<turnstile> P <: Q"} holds. By transitivity we obtain then 
+	@{term "(\<Delta>@[(X,P)]@\<Gamma>) \<turnstile> P <: N"} and can conclude by applying rule @{text "S_Var"}.
+	\end{minipage}*}
+      hence IH_inner: "(\<Delta>@[(X,P)]@\<Gamma>) \<turnstile> S <: N"
+	and lh_drv_prm: "(Y,S) \<in> set (\<Delta>@[(X,Q)]@\<Gamma>)"
+	and rh_drv: "\<Gamma> \<turnstile> P<:Q"
+	and ok\<^isub>Q: "\<turnstile> (\<Delta>@[(X,Q)]@\<Gamma>) ok" by (simp_all add: subtype_implies_ok)
+      hence ok\<^isub>P: "\<turnstile> (\<Delta>@[(X,P)]@\<Gamma>) ok" by (simp add: subtype_implies_ok) 
+      show "(\<Delta>@[(X,P)]@\<Gamma>) \<turnstile> Tvar Y <: N"
+      proof (cases "X=Y")
+	case False
+	have "X\<noteq>Y" by fact
+	hence "(Y,S)\<in>set (\<Delta>@[(X,P)]@\<Gamma>)" using lh_drv_prm by simp
+	with IH_inner show "(\<Delta>@[(X,P)]@\<Gamma>) \<turnstile> Tvar Y <: N" by (simp add: subtype_of.S_Var)
+      next
+	case True
+	have memb\<^isub>X\<^isub>Q: "(X,Q)\<in>set (\<Delta>@[(X,Q)]@\<Gamma>)" by simp
+	have memb\<^isub>X\<^isub>P: "(X,P)\<in>set (\<Delta>@[(X,P)]@\<Gamma>)" by simp
+	have eq: "X=Y" by fact 
+	hence "S=Q" using ok\<^isub>Q lh_drv_prm memb\<^isub>X\<^isub>Q by (simp only: uniqueness_of_ctxt)
 	hence "(\<Delta>@[(X,P)]@\<Gamma>) \<turnstile> Q <: N" using IH_inner by simp
 	moreover
 	have "(\<Delta>@[(X,P)]@\<Gamma>) extends \<Gamma>" by (simp add: extends_def)
-	hence "(\<Delta>@[(X,P)]@\<Gamma>) \<turnstile> P <: Q" using rh_drv cntxt_ok by (simp only: weakening)
-	ultimately have "(\<Delta>@[(X,P)]@\<Gamma>) \<turnstile> P <: N" using transitivity by simp
-	hence "(\<Delta>@[(X,P)]@\<Gamma>) \<turnstile> Tvar X <: N" using memb_XP cntxt_ok 
-	  by (simp only: subtype_of.S_Var)
-      }
-      ultimately show "(\<Delta>@[(X,P)]@\<Gamma>) \<turnstile> Tvar Y <: N" by blast
+	hence "(\<Delta>@[(X,P)]@\<Gamma>) \<turnstile> P <: Q" using rh_drv ok\<^isub>P by (simp only: weakening)
+	ultimately have "(\<Delta>@[(X,P)]@\<Gamma>) \<turnstile> P <: N" by (simp add: transitivity_aux) 
+	thus "(\<Delta>@[(X,P)]@\<Gamma>) \<turnstile> Tvar Y <: N" using memb\<^isub>X\<^isub>P eq by (simp only: subtype_of.S_Var)
+      qed
     next
       case (S_Refl _ Y \<Delta> \<Gamma> X)
-	--{* in this case lh drv is @{term "(\<Delta>@[(X,Q)]@\<Gamma>) \<turnstile> Tvar Y <: Tvar Y"} *}
-      hence lh_drv_prm1: "\<turnstile> (\<Delta>@[(X,Q)]@\<Gamma>) ok" 
-	and lh_drv_prm2: "Y \<in> domain (\<Delta>@[(X,Q)]@\<Gamma>)" by simp_all
+	--{* \begin{minipage}[t]{0.9\textwidth}
+	In this case the left-hand derivation is @{term "(\<Delta>@[(X,Q)]@\<Gamma>) \<turnstile> Tvar Y <: Tvar Y"} and we
+	therefore know that @{term "\<Delta>@[(X,Q)]@\<Gamma>"} is ok and thad @{term "Y"} is in 
+	the domain of @{term "\<Delta>@[(X,Q)]@\<Gamma>"}. We therefore know that @{term "\<Delta>@[(X,P)]@\<Gamma>"} is ok
+	and that @{term Y} is in the domain of @{term "\<Delta>@[(X,P)]@\<Gamma>"}. We can conclude by applying 
+	rule @{text "S_Refl"}.\end{minipage}*}
+      hence lh_drv_prm\<^isub>1: "\<turnstile> (\<Delta>@[(X,Q)]@\<Gamma>) ok" 
+	and lh_drv_prm\<^isub>2: "Y \<in> domain (\<Delta>@[(X,Q)]@\<Gamma>)" by simp_all
       have "\<Gamma> \<turnstile> P <: Q" by fact
       hence "P closed_in \<Gamma>" by (simp add: subtype_implies_closed)
-      with lh_drv_prm1 have "\<turnstile> (\<Delta>@[(X,P)]@\<Gamma>) ok" by (simp add: replace_type)
+      with lh_drv_prm\<^isub>1 have "\<turnstile> (\<Delta>@[(X,P)]@\<Gamma>) ok" by (simp add: replace_type)
       moreover
-      from lh_drv_prm2 have "Y \<in> domain (\<Delta>@[(X,P)]@\<Gamma>)" by (simp add: domain_append)
+      from lh_drv_prm\<^isub>2 have "Y \<in> domain (\<Delta>@[(X,P)]@\<Gamma>)" by (simp add: domain_append)
       ultimately show "(\<Delta>@[(X,P)]@\<Gamma>) \<turnstile> Tvar Y <: Tvar Y" by (simp add: subtype_of.S_Refl)
     next
-      case (S_Arrow _ Q1 Q2 S1 S2 \<Delta> \<Gamma> X) 
-	--{* in this case lh drv is @{term "(\<Delta>@[(X,Q)]@\<Gamma>) \<turnstile> Q1 \<rightarrow> Q2 <: S1 \<rightarrow> S2"} *}
-      thus "(\<Delta>@[(X,P)]@\<Gamma>) \<turnstile> Q1 \<rightarrow> Q2 <: S1 \<rightarrow> S2" by blast 
+      case (S_Arrow _ Q\<^isub>1 Q\<^isub>2 S\<^isub>1 S\<^isub>2 \<Delta> \<Gamma> X) 
+	--{* \begin{minipage}[t]{0.9\textwidth}
+	In this case the left-hand derivation is @{term "(\<Delta>@[(X,Q)]@\<Gamma>) \<turnstile> Q\<^isub>1 \<rightarrow> Q\<^isub>2 <: S\<^isub>1 \<rightarrow> S\<^isub>2"} 
+	and the proof is trivial.\end{minipage}*}
+      thus "(\<Delta>@[(X,P)]@\<Gamma>) \<turnstile> Q\<^isub>1 \<rightarrow> Q\<^isub>2 <: S\<^isub>1 \<rightarrow> S\<^isub>2" by blast 
     next
-      case (S_All _ Y S1 S2 T1 T2 \<Delta> \<Gamma> X)
-	--{* in this case lh drv is @{term "(\<Delta>@[(X,Q)]@\<Gamma>) \<turnstile> \<forall>[Y<:S1].S2 <: \<forall>[Y<:T1].T2"} *}
-      hence IH_inner1: "(\<Delta>@[(X,P)]@\<Gamma>) \<turnstile> T1 <: S1" 
-	and IH_inner2: "((Y,T1)#\<Delta>@[(X,P)]@\<Gamma>) \<turnstile> S2 <: T2" 
-	and lh_drv_prm2: "Y\<sharp>(\<Delta>@[(X,Q)]@\<Gamma>)" by force+
+      case (S_Forall _ Y S\<^isub>1 S\<^isub>2 T\<^isub>1 T\<^isub>2 \<Delta> \<Gamma> X)
+	--{* \begin{minipage}[t]{0.9\textwidth}
+	In this case teh left-hand derivation is @{text "(\<Delta>@[(X,Q)]@\<Gamma>) \<turnstile> \<forall>[Y<:S\<^isub>1].S\<^isub>2 <: \<forall>[Y<:T\<^isub>1].T\<^isub>2"}
+	and therfore we know that the binder @{term Y} is fresh for @{term "\<Delta>@[(X,Q)]@\<Gamma>"}. By
+	the inner induction hypothesis we have that @{term "(\<Delta>@[(X,P)]@\<Gamma>) \<turnstile> T\<^isub>1 <: S\<^isub>1"} and 
+	@{term "((Y,T\<^isub>1)#\<Delta>@[(X,P)]@\<Gamma>) \<turnstile> S\<^isub>2 <: T\<^isub>2"}. Since @{term P} is a subtype of @{term Q}
+	we can infer that @{term Y} is fresh for @{term P} and thus also fresh for 
+	@{term "\<Delta>@[(X,P)]@\<Gamma>"}. We can then conclude by applying rule @{text "S_Forall"}.
+	\end{minipage}*}
+      hence IH_inner\<^isub>1: "(\<Delta>@[(X,P)]@\<Gamma>) \<turnstile> T\<^isub>1 <: S\<^isub>1" 
+	and IH_inner\<^isub>2: "((Y,T\<^isub>1)#\<Delta>@[(X,P)]@\<Gamma>) \<turnstile> S\<^isub>2 <: T\<^isub>2" 
+	and lh_drv_prm: "Y\<sharp>(\<Delta>@[(X,Q)]@\<Gamma>)" by force+
       have rh_drv: "\<Gamma> \<turnstile> P <: Q" by fact
-      hence "Y\<sharp>P" using lh_drv_prm2 by (simp only: fresh_list_append subtype_implies_fresh)
-      hence "Y\<sharp>(\<Delta>@[(X,P)]@\<Gamma>)" using lh_drv_prm2 
+      hence "Y\<sharp>P" using lh_drv_prm by (simp only: fresh_list_append subtype_implies_fresh)
+      hence "Y\<sharp>(\<Delta>@[(X,P)]@\<Gamma>)" using lh_drv_prm 
 	by (simp add: fresh_list_append fresh_list_cons fresh_prod)
-      with IH_inner1 IH_inner2 
-      show "(\<Delta>@[(X,P)]@\<Gamma>) \<turnstile> \<forall>[Y<:S1].S2 <: \<forall>[Y<:T1].T2" by (simp add: subtype_of.S_All)
+      with IH_inner\<^isub>1 IH_inner\<^isub>2 
+      show "(\<Delta>@[(X,P)]@\<Gamma>) \<turnstile> \<forall>[Y<:S\<^isub>1].S\<^isub>2 <: \<forall>[Y<:T\<^isub>1].T\<^isub>2" by (simp add: subtype_of.S_Forall)
     qed
-  qed
-  from transitivity narrowing show ?case by blast 
+  } 
 qed
-
-
 
 
 end
